playground/play.v
@@ -1,0 +1,19 @@
+
+
+CoInductive itree (E : Type -> Type) (R : Type) : Type :=
+  | Ret (r : R)
+  | Tau (t : itree E R)
+  | Vis { A : Type } (e : E A) (k :  A -> itree E R).
+
+Inductive IO : Type -> Type := 
+  | Input : IO nat
+  | Output : nat -> IO unit.
+
+Inductive void := .
+
+CoFixpoint spin : itree IO void := Tau IO void spin.
+
+Check Tau.
+
+Context { E : Type -> Type } { A B : Type } (r : A -> B -> Prop).
+
